\documentclass{article}
\usepackage{geometry}
\usepackage[american]{babel}
\geometry{letterpaper}

\begin{document}

$\begin{array}{ll}
  B_j ( i) & = \sum_{k = 1}^{i - 1} e^{- \beta_j ( t_i - t_k)}\\
  & = e^{- \beta_j ( t_i - t_{i - 1})}_{} \sum_{k = 1}^{i - 1} e^{- \beta_j (
  t_{i - 1} - t_k)}\\
  & = e^{- \beta_j ( t_i - t_{i - 1})}_{}  \left( 1 + \sum_{k = 1}^{i - 2}
  e^{- \beta_j ( t_{i - 1} - t_k)} \right)\\
  & = e^{- \beta_j ( t - t_{i - 1})} ( 1 + B_j ( i - 1))
\end{array}$

\end{document}
