\documentclass{article}
\usepackage{geometry}
\usepackage[american]{babel}
\geometry{letterpaper}

%%%%%%%%%% Start TeXmacs macros
\newcommand{\mathd}{\mathrm{d}}
%%%%%%%%%% End TeXmacs macros

\begin{document}

$\begin{array}{ll}
  \Lambda ( t_{i - 1}, t_i) & = \int_{t_{i - 1}}^{t_i} \lambda ( t) \mathd t\\
  & = \int_{t_{i - 1}}^{t_i} \left( \lambda_0 ( t) + \sum_{j = 1}^P \alpha_j
  B_j ( N_t) \right) \mathd t\\
  & = \int_{t_{i - 1}^{}}^{t_i} \lambda_0 ( s) \mathd s + \int_{t_{i -
  1}^{}}^{t_i} \sum_{j = 1}^P \alpha_j \sum_{k = 0}^{i - 1} e^{- \beta_j ( t -
  t_k)} \mathd t\\
  & = \int_{t_{i - 1}^{}}^{t_i} \lambda_0 ( s) \mathd s + \sum_{j = 1}^P
  \alpha_j \sum_{k = 0}^{i - 1}  \int_{t_{i - 1}^{}}^{t_i} e^{- \beta_j ( t -
  t_k)} \mathd t\\
  & = \int_{t_{i - 1}^{}}^{t_i} \lambda_0 ( s) \mathd s + \sum_{k = 0}^{i -
  1} \int_{t_{i - 1}}^{t_i} \nu ( t - t_k) \mathd t\\
  & = \int_{t_{i - 1}^{}}^{t_i} \lambda_0 ( s) \mathd s + \sum_{k = 0}^{i -
  1} \sum_{j = 1}^P \frac{\alpha_j}{\beta_j} ( e^{- \beta_j ( t_{i - 1} -
  t_k)} - e^{- \beta_j ( t_i - t_k)})\\
  & = \int_{t_{i - 1}^{}}^{t_i} \lambda_0 ( s) \mathd s + \sum_{j = 1}^P
  \frac{\alpha_j}{\beta_j} ( 1 - e^{- \beta_j ( t_i - t_{i - 1})}) A_j ( i -
  1)
\end{array}$

\end{document}
